Almost done with the Coqing

part3/src/Queue.v
@@ -1,17 +1,30 @@
-Require Import List.
+Require Import Arith List.
 
 Module Type QUEUE.
   Parameter Q : Type -> Type.
-  
+  Parameter inv : forall A, Q A -> Prop.
   Parameter empty  : forall A, Q A.
   Parameter inject : forall A, A -> Q A -> Q A.
   Parameter pop    : forall A, Q A -> Q A.
-  Parameter peak   : forall A, Q A -> option A.
-
+  Parameter peak   : forall A, Q A -> option A.  
   Parameter to_list : forall A, Q A -> list A.
-
+  
   Definition represents {A : Type} (q : Q A) (l : list A) : Prop :=
     to_list _ q = l.
+
+  Axiom empty_inv :
+    forall A, 
+      inv A (empty A).
+
+  Axiom inject_inv :
+    forall A q x,
+      inv A q ->
+      inv _ (inject _ x q).
+
+  Axiom pop_inv :
+    forall A q,
+      inv A q ->
+      inv _ (pop _ q).
   
   Axiom empty_is_empty : forall A,
     represents (empty A) nil.
@@ -19,30 +32,40 @@ Module Type QUEUE.
   Axiom inject_spec :
     forall A l q x,
       represents q l ->
+      inv _ q ->
       represents (inject A x q) (l ++ (x :: nil)).
   
   Axiom pop_empty :
     forall A q,
       represents q nil ->
+      inv _ q ->
       represents (pop A q) nil.
+
   Axiom pop_xs :
     forall A q x xs,
       represents q (x::xs) ->
+      inv _ q ->
       represents (pop A q) xs.
   
   Axiom peak_empty_spec :
     forall A q,
       represents q nil ->
+      inv _ q -> 
       peak A q = None.
+
   Axiom peak_spec :
     forall A q x xs,
       represents q (x::xs) ->
+      inv _ q ->
       peak A q = Some x.
+
 End QUEUE.
 
 Module BasicQueue <: QUEUE.
 
   Definition Q := list.
+
+  Definition inv := fun (A : Type) (q : Q A) => True.
 
   Definition empty := @nil.
 
@@ -67,16 +90,35 @@ Module BasicQueue <: QUEUE.
       | nil => nil
       | _ :: q' => q'
     end.
+
   Definition peak {A : Type} (q : Q A) :=
     match q with
       | nil => None
       | x :: _ => Some x
     end.
+
   Definition to_list {A : Type} (q : Q A) := q.
   
   Definition represents {A : Type} (q : Q A) (l : list A) : Prop :=
     to_list q = l.
 
+  Lemma empty_inv : 
+    forall A,
+      inv A (empty A).
+  Proof. constructor. Qed.
+
+  Lemma inject_inv :
+    forall A q x,
+      inv A q ->
+      inv _ (inject x q).
+  Proof. constructor. Qed.
+
+  Lemma pop_inv : 
+    forall A q,
+      inv A q ->
+      inv _ (pop q).
+  Proof. constructor. Qed.
+ 
   Lemma empty_is_empty : forall A,
     represents (empty A) nil.
   Proof.
@@ -89,6 +131,7 @@ Module BasicQueue <: QUEUE.
   Lemma inject_spec :
     forall A l q (x : A),
       represents q l ->
+      inv _ q ->
       represents (inject x q) (l ++ (x :: nil)).
   Proof.
     unfold represents, to_list.
@@ -104,11 +147,13 @@ Module BasicQueue <: QUEUE.
     rewrite app_comm_cons.
     reflexivity.
     reflexivity.
+    constructor.
   Qed.
 
   Lemma pop_empty :
     forall A (q : Q A),
       represents q nil ->
+      inv _ q ->
       represents (pop q) nil.
   Proof.
     unfold represents, to_list.
@@ -119,7 +164,8 @@ Module BasicQueue <: QUEUE.
 
   Lemma pop_xs :
     forall A (q : Q A) x xs,
-      represents q (x::xs) ->
+      represents q (x::xs) ->      
+      inv _ q ->
       represents (pop q) xs.
   Proof.
     unfold represents, to_list.
@@ -132,6 +178,7 @@ Module BasicQueue <: QUEUE.
   Lemma peak_empty_spec :
     forall A (q : Q A),
       represents q nil ->
+      inv _ q ->
       peak q = None.
   Proof.
     unfold represents, to_list.
@@ -143,6 +190,7 @@ Module BasicQueue <: QUEUE.
   Lemma peak_spec :
     forall A (q : Q A) x xs,
       represents q (x::xs) ->
+      inv _ q -> 
       peak q = Some x.
   Proof.
     unfold represents, to_list.
@@ -154,3 +202,464 @@ Module BasicQueue <: QUEUE.
 
 End BasicQueue.
 
+Module PairQueue <: QUEUE.
+
+  Definition Q := fun A : Type => ((list A) * (list A))%type.
+
+  Definition inv := fun (A : Type) (q : Q A) => True.
+
+  Definition empty {A : Type} := (@nil A, @nil A).
+
+  Definition inject {A : Type} (a : A) (q : Q A) := 
+    match q with
+      | (h, t) => (h, a :: t)
+    end.
+
+  Definition pop {A : Type} (q : Q A) :=
+    match q with
+      | (h, t) => 
+        match h with
+          | (_ :: h') => (h', t)
+          | nil =>
+            match rev t with
+              | nil => (nil, nil)
+              | (_ :: t') => (t', nil)
+            end
+        end
+    end.
+
+  Definition peak {A : Type} (q : Q A) : option A :=
+    match q with
+      | (h, t) =>
+        match h with
+          | (x :: _) => Some x
+          | nil =>
+            match rev t with
+              | nil => None
+              | (x :: _) => Some x
+            end
+        end
+    end.
+
+  Definition to_list {A : Type} (q : Q A) :=
+    match q with
+      | (h, t) => h ++ rev t
+    end.
+
+  Definition represents {A : Type} (q : Q A) (l : list A) : Prop :=
+    to_list q = l.
+
+    Lemma empty_inv : 
+    forall A,
+      inv A (@empty A).
+  Proof. constructor. Qed.
+
+  Lemma inject_inv :
+    forall A q x,
+      inv A q ->
+      inv _ (inject x q).
+  Proof. constructor. Qed.
+
+  Lemma pop_inv : 
+    forall A q,
+      inv A q ->
+      inv _ (pop q).
+  Proof. constructor. Qed.
+
+  
+  Lemma empty_is_empty : forall A,
+    represents (@empty A) nil.
+  Proof.
+    unfold represents.
+    unfold to_list.
+    unfold empty.
+    reflexivity.
+  Qed.
+
+  Lemma inject_spec :
+    forall A l q (x : A),
+      represents q l ->
+      inv _ q -> 
+      represents (inject x q) (l ++ (x :: nil)).
+  Proof.
+    unfold represents, to_list. 
+    intros.
+    destruct q as (h, t).
+    unfold inject.
+    simpl.
+    rewrite app_assoc.
+    rewrite H.
+    reflexivity.
+  Qed.
+
+  Lemma pop_empty :
+    forall A (q : Q A),
+      represents q nil ->
+      inv _ q ->
+      represents (pop q) nil.
+  Proof.
+    unfold represents, to_list, pop.
+    intros.
+    destruct q as (h, t).
+    destruct h.
+    destruct (rev t).
+    reflexivity.
+    inversion H.        
+    inversion H.
+  Qed.      
+  
+  Lemma pop_xs :
+    forall A (q : Q A) x xs,
+      represents q (x::xs) ->
+      inv _ q -> 
+      represents (pop q) xs.
+  Proof.
+    unfold represents, to_list.
+    intros.
+    destruct q as (h, t).
+    unfold pop.
+    
+    destruct h.
+    destruct (rev t).
+    inversion H.
+    inversion H.
+    simpl.
+    rewrite app_nil_r.
+    reflexivity.
+    inversion H.
+    reflexivity.    
+  Qed.
+  
+  Lemma peak_empty_spec :
+    forall A (q : Q A),
+      represents q nil ->
+      inv _ q -> 
+      peak q = None.
+  Proof.
+    unfold represents, to_list.
+    intros.
+    destruct q as (h, t).
+    apply app_eq_nil in H.
+    destruct H as [Hh Ht].
+    unfold peak.
+    rewrite Hh, Ht.
+    reflexivity.
+  Qed.
+
+  Lemma peak_spec :
+    forall A (q : Q A) x xs,
+      represents q (x::xs) ->
+      inv _ q ->
+      peak q = Some x.
+  Proof.
+    unfold represents, to_list.
+    destruct q as (h, t).
+    intros.
+    destruct h.
+    simpl in H.
+    unfold peak.
+    rewrite H.
+    reflexivity.
+    unfold peak.
+    inversion H.
+    reflexivity.
+  Qed.  
+End PairQueue.
+
+Module OkasakiQueue <: QUEUE.
+
+  Definition Q (A : Type) :=
+    (list A * list A)%type.
+  
+  Definition inv (A : Type) (q : Q A) : Prop :=
+    let (h, t) := q in
+    leb (length t) (length h) = true.
+
+  Definition empty {A : Type} := 
+    (@nil A, @nil A).
+
+  Definition inject {A : Type} (a : A) (q : Q A) :=
+    let (h, t) := q in
+    if andb (leb (length t) (length h)) (negb (beq_nat (length t) (length h)))
+    then (h, a :: t)
+    else (h ++ rev (a :: t), nil).
+
+  Definition pop {A : Type} (q : Q A) : Q A :=
+    let (h, t) := q in
+    match h with
+      | nil => (nil, nil)
+      | (e :: h') => 
+        if beq_nat (length h) (length t)
+        then (h' ++ rev t, nil)
+        else (h', t)
+    end.
+ 
+  Definition peak {A : Type} (q : Q A) : option A :=
+    let (h, t) := q in
+    match h with
+      | nil => None
+      | e :: _ => Some e
+    end.
+
+  Definition to_list {A : Type} (q : Q A) :=
+    let (h, t) := q in
+    h ++ rev t.
+  
+  Definition represents {A : Type} (q : Q A) (l : list A) : Prop :=
+    to_list q = l.
+
+  Lemma empty_inv :
+    forall A, 
+      inv A (@empty A).
+  Proof.
+    intro A.
+    unfold inv.
+    unfold empty.
+    simpl.
+    reflexivity.
+  Qed.
+      
+  Lemma inject_inv :
+    forall A q x,
+      inv A q ->
+      inv _ (inject x q).
+  Proof.
+    unfold inv.
+    destruct q as (h, t); intros.
+    unfold inject.
+    remember (beq_nat (length t) (length h)) as hvt.
+    destruct hvt.
+    rewrite H.
+    reflexivity.
+    rewrite H.
+    simpl.
+    destruct (length h).
+    symmetry in Heqhvt.
+    apply beq_nat_false in Heqhvt.
+    apply leb_complete in H.
+    inversion H.
+    contradiction.
+    apply leb_complete in H.
+    symmetry in Heqhvt.
+    apply beq_nat_false in Heqhvt.
+    apply NPeano.Nat.le_succ_r in H.
+    destruct H.
+    apply leb_correct.
+    assumption.
+    contradiction.
+  Qed.
+
+  Lemma pop_inv :
+    forall A q,
+      inv A q ->
+      inv _ (pop q).
+  Proof.
+    unfold inv, pop.
+    destruct q as (h, t).
+    intros.
+    destruct h.
+    reflexivity.
+    remember (beq_nat (length (a :: h)) (length t)) as hvt.
+    destruct hvt.
+    reflexivity.
+    apply leb_correct.
+    apply leb_complete in H.
+    simpl in H.
+    symmetry in Heqhvt.
+    apply beq_nat_false in Heqhvt.
+    simpl in Heqhvt.
+    apply NPeano.Nat.le_succ_r in H.
+    destruct H.
+    assumption.
+    symmetry in H.
+    contradiction.
+  Qed.
+
+  Lemma empty_is_empty : forall A,
+    represents (@empty A) nil.
+  Proof. reflexivity. Qed.
+  
+  Lemma inject_spec :
+    forall A l q x,
+      represents q l ->
+      inv A q ->
+      represents (inject x q) (l ++ (x :: nil)).
+  Proof.
+    unfold represents, to_list, inv.
+    destruct q as (h, t).    
+    intros.
+    unfold inject.
+    rewrite H0.
+    simpl.
+    destruct (beq_nat (length t) (length h)); simpl.    
+    rewrite app_nil_r.
+    rewrite app_assoc.
+    rewrite H.
+    reflexivity.
+    rewrite app_assoc.
+    rewrite H.
+    reflexivity.
+  Qed.
+
+  Lemma pop_empty :
+    forall A q,
+      represents q nil ->
+      inv A q ->
+      represents (pop q) nil.
+  Proof.
+    unfold represents, to_list, inv.
+    destruct q as (h, t).
+    intros.
+    apply app_eq_nil in H.
+    destruct H as [Hh Ht].
+    unfold pop.
+    rewrite Hh.
+    reflexivity.
+  Qed.
+
+  Lemma length_O_is_nil :
+    forall A xs,
+      length xs = 0 ->
+      xs = @nil A.
+  Proof.
+    induction xs; intros.
+    reflexivity.
+    inversion H.
+  Qed.
+
+  Lemma pop_xs :
+    forall A q x xs,
+      represents q (x::xs) ->
+      inv A q ->
+      represents (pop q) xs.
+  Proof.
+    unfold represents, to_list, inv.
+    destruct q as (h, t).
+    intros.
+    unfold pop.
+    destruct h.
+    simpl in H, H0.
+    apply leb_complete in H0.
+    inversion H0.
+    apply length_O_is_nil in H2.
+    rewrite H2 in H.
+    inversion H.
+    inversion H.
+    destruct (beq_nat (length (x :: h)) (length t)).
+    rewrite app_nil_r.
+    reflexivity.
+    reflexivity.
+  Qed.
+
+  Lemma peak_empty_spec :
+    forall A q,
+      represents q nil ->
+      inv A q -> 
+      peak q = None.
+  Proof.
+    unfold represents, to_list, inv, peak.
+    destruct q as (h, t).
+    intros.
+    destruct h.
+    reflexivity.
+    inversion H.
+  Qed.
+
+  Lemma peak_spec :
+    forall A q x xs,
+      represents q (x::xs) ->
+      inv A q ->
+      peak q = Some x.
+  Proof.
+    unfold represents, to_list, inv, peak.
+    destruct q as (h, t).
+    intros.
+    destruct h.
+    simpl in H0.
+    apply leb_complete in H0.
+    inversion H0.
+    apply length_O_is_nil in H2.
+    rewrite H2 in H.
+    inversion H.
+    inversion H.
+    reflexivity.
+  Qed.
+End OkasakiQueue.
+
+Module HoodMelvilleQueue <: QUEUE.
+  
+  Definition Q (A : Type) :=
+    (nat * nat * list A * list A * list A * list A * list A * list A)%type.
+  
+  Definition inv {A : Type} (q : Q A) : Prop :=
+    match q with  
+      | (p, s, f, a, b, c, d, e) =>
+        (length e + p) <= (length d + (NPeano.div (length a) 2))
+        /\ NPeano.div (2 * length b + length a + length c) 3 <= length f
+        /\ length f = length b + (s - p)
+    end.
+
+  Definition empty {A : Type} :=
+    (0, 0, @nil A, @nil A, @nil A, @nil A, @nil A, @nil A).
+
+  Definition fix {A : Type} :=
+    match q with  
+      | (p, s, f, a, b, c, d, e) =>
+        
+
+  Definition inject : forall A, A -> Q A -> Q A.
+  Parameter pop    : forall A, Q A -> Q A.
+  Parameter peak   : forall A, Q A -> option A.  
+  Parameter to_list : forall A, Q A -> list A.
+  
+  Definition represents {A : Type} (q : Q A) (l : list A) : Prop :=
+    to_list _ q = l.
+
+  Axiom empty_inv :
+    forall A, 
+      inv A (empty A).
+
+  Axiom inject_inv :
+    forall A q x,
+      inv A q ->
+      inv _ (inject _ x q).
+
+  Axiom pop_inv :
+    forall A q,
+      inv A q ->
+      inv _ (pop _ q).
+  
+  Axiom empty_is_empty : forall A,
+    represents (empty A) nil.
+  
+  Axiom inject_spec :
+    forall A l q x,
+      represents q l ->
+      inv _ q ->
+      represents (inject A x q) (l ++ (x :: nil)).
+  
+  Axiom pop_empty :
+    forall A q,
+      represents q nil ->
+      inv _ q ->
+      represents (pop A q) nil.
+
+  Axiom pop_xs :
+    forall A q x xs,
+      represents q (x::xs) ->
+      inv _ q ->
+      represents (pop A q) xs.
+  
+  Axiom peak_empty_spec :
+    forall A q,
+      represents q nil ->
+      inv _ q -> 
+      peak A q = None.
+
+  Axiom peak_spec :
+    forall A q x xs,
+      represents q (x::xs) ->
+      inv _ q ->
+      peak A q = Some x.
+
+End QUEUE.
